Spec/Async.s.dfy
@@ -1,0 +1,49 @@
+include "AtomicStateMachine.s.dfy"
+
+module AsyncMod(atomic: AtomicStateMachineMod) {
+  type ID(==, !new)
+  datatype Request = Request(input: atomic.Input, id: ID)
+  datatype Reply = Reply(output: atomic.Output, id: ID)
+
+  datatype Variables = Variables(mapv: atomic.Variables, requests: set<Request>, replies: set<Reply>)
+
+  function InitState() : Variables {
+    Variables(atomic.InitState(), {}, {})
+  }
+
+  predicate DoRequest(v: Variables, v': Variables, req: Request) {
+    // TODO Probably should disallow ID conflicts
+    && v' == v.(requests := v.requests + {req})
+  }
+
+  // The serialization point for this request
+  predicate DoExecute(v: Variables, v': Variables, req: Request, reply: Reply) {
+    && reply.id == req.id
+    && req in v.requests
+    && atomic.Next(v.mapv, v'.mapv, req.input, reply.output)
+    && v'.requests == v.requests - {req}
+    && v'.replies == v.replies + {reply}
+  }
+
+  predicate DoReply(v: Variables, v': Variables, reply: Reply)
+  {
+    && reply in v.replies
+    && v' == v.(replies := v.replies - {reply})
+  }
+
+  datatype UIOp =
+    | RequestOp(req: Request)
+    | ExecuteOp(req: Request, reply: Reply)
+    | ReplyOp(reply: Reply)
+
+  predicate NextStep(v: Variables, v': Variables, op: UIOp) {
+    match op
+      case RequestOp(req) => DoRequest(v, v', req)
+      case ExecuteOp(req, reply) => DoExecute(v, v', req, reply)
+      case ReplyOp(reply) => DoReply(v, v', reply)
+  }
+
+  predicate Next(v: Variables, v': Variables) {
+    exists step :: NextStep(v, v', step)
+  }
+}
