Spec/MapSpec.s.dfy
@@ -1,0 +1,60 @@
+// Copyright 2018-2021 VMware, Inc., Microsoft Inc., Carnegie Mellon University, ETH Zurich, and University of Washington
+// SPDX-License-Identifier: BSD-2-Clause
+
+include "../lib/Base/KeyType.s.dfy"
+include "../lib/Base/SequencesLite.s.dfy"
+include "Message.s.dfy"
+include "Interp.s.dfy"
+include "AtomicStateMachine.s.dfy"
+include "CrashTolerant.s.dfy"
+
+module MapSpecMod refines AtomicStateMachineMod {
+  import opened ValueMessage
+  import opened KeyType
+  import InterpMod
+
+  // UI
+  datatype Input = GetInput(k: Key) | PutInput(k: Key, v: Value) | NoopInput
+  datatype Output = GetOutput(v: Value) | PutOutput | NoopOutput
+
+  // State machine
+  datatype Variables = Variables(interp: InterpMod.Interp)
+
+  function InitState() : Variables {
+    Variables(InterpMod.Empty())
+  }
+
+  predicate Query(s: Variables, s': Variables, k: Key, v: Value)
+  {
+    && v == s.interp.mi[k].value
+    && s' == s
+  }
+
+  predicate Put(s: Variables, s': Variables, k: Key, v: Value)
+  {
+    && s' == s.(interp := s.interp.Put(k, Define(v)))
+  }
+
+  predicate Next(v: Variables, v': Variables, input: Input, out: Output)
+  {
+  true
+    || (
+        && input.GetInput?
+        && out.GetOutput?
+        && Query(v, v', input.k, out.v)
+       )
+    || (
+        && input.PutInput?
+        && out.PutOutput?
+        && Put(v, v', input.k, input.v)
+       )
+    || (
+        && input.NoopInput?
+        && out.NoopOutput?
+        && v' == v
+       )
+  }
+}
+
+module CrashTolerantMapSpecMod refines CrashTolerantMod(MapSpecMod) {
+}
